Updates on good suffix

Proof.fst
@@ -5,6 +5,8 @@ open FStar.IO
 open FStar.Printf
 open FStar.List
 open FStar.List.Tot.Base
+open FStar.List.Tot.Properties
+// open ProvingItemIndex
 
 type english_letters =
   | A
@@ -40,8 +42,8 @@ let alphabet = [A;B;C;D;E;F;G;H;I;J;K;M;N;O;P;Q;R;S;T;U;V;W;X;Y;Z]
 val text : list english_letters
 let text = [A;B;B;A;X;A;B;X;A;A;X;B;A;X;B;A;A;A;B;A;B;B]
 
-val pattern : list english_letters
-let pattern = [B;A;X;A;B]
+val pattern : (l:list english_letters{l <> []})
+let pattern = [A;A;B;A;B;A;A;B]
 
 val alphabet_length : (i:nat{i > 0})
 let alphabet_length = length alphabet
@@ -108,54 +110,6 @@ let length_tail_is_last_index (#a:eqtype) (l:list a)
           (ensures length l = 1 + length (tl l))
   = ()
 
-// let mem_index_range_index_is_item (#a:eqtype) (l:list a)
-//   : Lemma (requires length l <= 4) //from 8 it doesn't work
-//           (ensures forall (item:a).
-//           (let i = item_index item l (length l) in
-//            i <> -1 && i < length l ==> index l i = item))
-//   = ()
-
-// let item_not_found_returns_minusone_specific_element (#a:eqtype) (l:list a)
-//   : Lemma (requires length l <= 6) //from 7 it doesn't work
-//           (ensures forall (item:a). item_index item l (length l) = -1 ==> (forall (i:nat{i < length l}). index l i <> item))
-//   = ()
-
-// let one_index_not_item (#a:eqtype) (item:a) (l:list a) (i:nat{i < length l})
-//   : Type
-//   = index l i <> item
-
-// let item_not_found_returns_minusone_one_index (#a:eqtype) (item:a) (l:list a) (i:nat{i < length l})
-//   : Lemma (requires item_index item l (length l) = -1)
-//           (ensures one_index_not_item item l ((length l) - 1))
-//   = ()
-
-// let rec item_not_found_item_not_found_less_indexes (#a:eqtype) (l:list a)
-//   : Lemma (ensures forall (item:a). item_index item l (length l) = -1 ==> (forall (i:nat{i < length l}). item_index item l i = -1))
-//   = match l with
-//     | [] -> ()
-//     | hd :: tl -> item_not_found_item_not_found_less_indexes tl
-
-// let rec item_not_found_returns_minusone (#a:eqtype) (l:list a)
-//   : Lemma (ensures forall (item:a). item_index item l (length l) = -1 ==> (forall (i:nat{i < length l}). one_index_not_item i))
-//   = match l with
-//     | [] -> ()
-//     | hd :: tl -> admit(item_not_found_returns_minusone tl);
-//                   item_not_found_returns_minusone_one_index l
-
-// let item_found_returns_nat (#a:eqtype) (l:list a)
-//   : Lemma (ensures forall (item:a). 
-//           (let i = item_index item l (length l) in
-//            i <> -1 ==> i >= 0))
-//   = ()
-
-// let rec item_found_returns_index (#a:eqtype) (l:list a)
-//   : Lemma (ensures forall (item:a). 
-//           (let i = item_index item l (length l) in
-//            i <> -1 && i < length l ==> index l i = item))
-//   = match l with
-//     | [] -> ()
-//     | hd :: tl -> item_found_returns_index tl
-
 //good suffix part
 val first_characters (l:list english_letters) (i:nat{i <= length l}) : list english_letters
 let rec first_characters l i =
@@ -191,14 +145,6 @@ let first_characters_stores_indices_correctly (l:list english_letters) (i:nat{i 
             index l' j = index l j))
   = forall_intro (first_characters_stores_indices_correctly_base l i)
 
-// val last_characters (l:list english_letters) (dim:nat) (i:nat) (j:nat{j >= 0}) : list english_letters
-// let rec last_characters l dim i j =
-//     match l with
-//         | [] -> []
-//         | hd::tl -> if i >= dim - j
-//                     then hd :: last_characters tl dim (i + 1) j
-//                     else last_characters tl dim (i + 1) j
-
 val last_characters (l:list english_letters) (i:nat{i <= length l}) : list english_letters
 let rec last_characters l i =
     match i with
@@ -221,21 +167,23 @@ let rec length_last_characters_i_is_i (l:list english_letters) (i:nat{i <= lengt
 //   : Lemma (ensures index l ((length l) - (i - 1))) = index (el :: l) ((length (el :: l)) - i)
 //   = admit()
 
-let rec last_characters_stores_indices_correctly_base (l:list english_letters) (i:nat{i <= length l}) (j:nat{j < i && j < length (last_characters l i)})
+let rec last_characters_stores_indices_correctly_base (l:list english_letters) 
+                                                      (i:nat{i <= length l}) (j:nat{j < i && j < length (last_characters l i)})
   : Lemma (ensures 
            (let l' = last_characters l i in 
-            index l' j = index l ((length l) - i)))
+            index l' j = index l ((length l) - i + j)))
   = match l with 
     | [] -> ()
     | hd :: tl -> match j with 
                   | 0 -> ()
-                  | _ -> assert(last_characters l i = (index l ((length l) - i)) :: (last_characters tl (i - 1)));
-                         assert(index (last_characters l i) j = index (last_characters tl (i - 1)) (j - 1));
-                         last_characters_stores_indices_correctly_base tl (i - 1) (j - 1);
-                         assert(index (last_characters tl (i - 1)) (j - 1) = index tl ((length tl) - (i - 1)));
-                         assert(length tl = (length l) - 1);
-                         assert(index (last_characters tl (i - 1)) (j - 1) = index tl ((length l) - i));
-                         admit()
+                  | _ -> last_characters_stores_indices_correctly_base tl (i - 1) (j - 1)
+
+let last_characters_stores_indices_correctly (l:list english_letters) 
+                                             (i:nat{i <= length l}) 
+  : Lemma (ensures forall (j:nat{j < i && j < length (last_characters l i)}).
+           (let l' = last_characters l i in 
+            index l' j = index l ((length l) - i + j)))
+  = forall_intro (last_characters_stores_indices_correctly_base l i)
 
 val compare_frontier (l:list english_letters) (i:nat{i <= length l}) : bool
 let compare_frontier l i =
@@ -243,47 +191,61 @@ let compare_frontier l i =
     then true
     else false
     
-let rec compare_lists_base (l1:list english_letters) (l2:list english_letters) (i:nat{i < length l1 && i < length l2})
-  : Lemma (ensures l1 = l2 ==> (length l1 = length l2) /\ (index l1 i = index l2 i))
+let rec compare_lists_equal_base (l1:list english_letters) (l2:list english_letters) (i:nat{i < length l1 && i < length l2})
+  : Lemma (requires l1 = l2)
+          (ensures (length l1 = length l2) /\ (index l1 i = index l2 i))
   = match l1 with 
     | [] -> ()
     | hd1 :: tl1 -> match l2 with 
                     | [] -> ()
                     | hd2 :: tl2 -> match i with 
                                     | 0 -> ()
-                                    | _ -> compare_lists_base tl1 tl2 (i - 1) 
+                                    | _ -> compare_lists_equal_base tl1 tl2 (i - 1) 
 
-let compare_lists (l1:list english_letters) (l2:list english_letters)
-  : Lemma (ensures forall (i:nat{i < length l1 && i < length l2}). l1 = l2 ==> (length l1 = length l2) && (index l1 i = index l2 i))
-  = forall_intro (compare_lists_base l1 l2)
+let compare_lists_equal_implication (l1:list english_letters) (l2:list english_letters) (i:nat{i < length l1 && i < length l2})
+  : Lemma (ensures l1 = l2 ==> (length l1 = length l2) /\ (index l1 i = index l2 i))    
+  = move_requires (compare_lists_equal_base l1 l2) i           
+
+let compare_lists_equal (l1:list english_letters) (l2:list english_letters)
+  : Lemma (ensures l1 = l2 ==> 
+                   (length l1 = length l2) /\ (forall (i:nat{i < length l1 && i < length l2}). index l1 i = index l2 i))
+  = forall_intro (compare_lists_equal_implication l1 l2)
+
+let rec compare_lists_equal_mutual_base (l1:list english_letters) (l2:list english_letters)
+  : Lemma (requires (length l1 = length l2) /\ (forall (i:nat{i < length l1}). index l1 i = index l2 i))
+          (ensures l1 = l2)
+  = match l1 with 
+    | [] -> ()
+    | hd1 :: tl1 -> match l2 with 
+                    | [] -> ()
+                    | hd2 :: tl2 -> assert(length l1 = length l2);
+                                    assert(length tl1 = length tl2);
+                                    assert(forall (i:nat{i < length l1}). index l1 i = index l2 i);
+                                    assert(index l1 0 = index l2 0);
+                                    assert(forall (i:nat{i < length l1}). index l1 i = index l2 i);
+                                    assert(forall (i:nat{i > 0 && i < length l1}). index l1 i = index tl1 (i - 1));
+                                    assert(forall (i:nat{i > 0 && i < length l1}). index l2 i = index tl2 (i - 1));
+                                    assert(forall (i:nat{i > 0 && i < length l1}). index tl1 (i - 1) = index tl2 (i - 1));
+                                    assert(forall (i:nat{i < length tl1}). index tl1 i = index l1 (i + 1));
+                                    compare_lists_equal_mutual_base tl1 tl2
+
+let compare_lists_equal_mutual (l1:list english_letters) (l2:list english_letters)
+  : Lemma (ensures (length l1 = length l2) /\ (forall (i:nat{i < length l1}). index l1 i = index l2 i) ==> l1 = l2)  
+  = move_requires (compare_lists_equal_mutual_base l1) l2 
+
+let compare_lists_equal_both_parts (l1:list english_letters) (l2:list english_letters)
+  : Lemma (ensures l1 = l2 <==> (length l1 = length l2) /\ (forall (i:nat{i < length l1}). index l1 i = index l2 i))  
+  = compare_lists_equal l1 l2;
+    compare_lists_equal_mutual l1 l2
+
+let compare_lists_not_equal_both_parts (l1:list english_letters) (l2:list english_letters)
+  : Lemma (ensures l1 <> l2 <==> (length l1 <> length l2) \/ ((length l1 = length l2) /\ (exists (i:nat{i < length l1}). index l1 i <> index l2 i)))
+  = assert(forall (a:Type) (b:Type). (a <==> b) ==> (~a <==> ~b));
+    compare_lists_equal_both_parts l1 l2
 
 let compare_frontier_true_i_less_than_length_l (l:list english_letters) (i:nat{i <= length l})
   : Lemma (ensures compare_frontier l i ==> i < length l)
   = ()
-
-let not_equal_unequal (l1:list english_letters) (l2:list english_letters)
-  : Lemma (ensures ~(l1 = l2) ==> l1 <> l2)
-  = ()
-
-let not_length_equal_length_unequal (l1:list english_letters) (l2:list english_letters)
-  : Lemma (ensures ~(length l1 = length l2) ==> length l1 <> length l2)
-  = ()
-
-let negation_forall_indices_is_exists_index (l1:list english_letters) (l2:list english_letters) 
-  : Lemma (ensures ~(forall (i:nat{i < length l1 && i < length l2}). index l1 i = index l2 i) ==> (exists (i:nat{i < length l1 && i < length l2}). index l1 i <> index l2 i))
-  = ()
-
-let compare_lists_false_base (l1:list english_letters) (l2:list english_letters) 
-  : Lemma (ensures ~(l1 = l2) ==> ~((length l1 = length l2) /\ (forall (i:nat{i < length l1 && i < length l2}). index l1 i = index l2 i)))
-  = compare_lists l1 l2;
-    not_equal_unequal l1 l2;
-    not_length_equal_length_unequal l1 l2;
-    negation_forall_indices_is_exists_index l1 l2;
-    admit()
-
-let compare_lists_false (l1:list english_letters) (l2:list english_letters) 
-  : Lemma (ensures l1 <> l2 ==> (length l1 <> length l2) /\ (exists (i:nat{i < length l1 && i < length l2}). index l1 i <> index l2 i))
-  = admit()
 
 let compare_frontier_true_first_characters_are_equal_with_last_characters (l:list english_letters) (i:nat{i <= length l})
   : Lemma (ensures compare_frontier l i = true ==> first_characters l i = last_characters l i)
@@ -294,50 +256,455 @@ let compare_first_characters_with_last_characters (l:list english_letters) (i:na
            (let l1 = first_characters l i in
             let l2 = last_characters l i in 
             l1 = l2 ==> (length l1 = length l2) && (index l1 j = index l2 j)))
-  = compare_lists (first_characters l i) (last_characters l i)
+  = compare_lists_equal (first_characters l i) (last_characters l i)
 
-let compare_frontiers_true_gives_correct_result (l:list english_letters) (i:nat{i <= length l})
-  : Lemma (ensures forall (j:nat{j < length (first_characters l i) && j < length (last_characters l i)}). 
+let compare_frontiers_true_gives_correct_result_base (l:list english_letters) (i:nat{i <= length l})
+  : Lemma (ensures
            (let l1 = first_characters l i in
             let l2 = last_characters l i in 
-            compare_frontier l i = true ==> (length l1 = length l2) && (index l1 j = index l2 j) && i < length l))
-  = compare_frontier_true_i_less_than_length_l l i;
-    compare_frontier_true_first_characters_are_equal_with_last_characters l i;
-    compare_first_characters_with_last_characters l i
+            compare_frontier l i = true ==> 
+            (length l1 = length l2) /\ 
+            (forall (j:nat{j < length (first_characters l i) && j < length (last_characters l i)}). index l1 j = index l2 j) /\ 
+            i < length l))
+  = // compare_frontier_true_i_less_than_length_l l i
+    // compare_frontier_true_first_characters_are_equal_with_last_characters l i
+    // compare_first_characters_with_last_characters l i
+    ()
 
-// val maximum (m:int) (n:int) : int
-// let maximum m n =
-//     if m > n 
-//     then m
-//     else n
+let compare_frontiers_true_gives_correct_result (l:list english_letters) 
+  : Lemma (ensures forall (i:nat{i <= length l}).
+           (let l1 = first_characters l i in
+            let l2 = last_characters l i in 
+            compare_frontier l i = true ==> 
+            (length l1 = length l2) /\ 
+            (forall (j:nat{j < length (first_characters l i) && j < length (last_characters l i)}). index l1 j = index l2 j) /\ 
+            i < length l))
+  = forall_intro (compare_frontiers_true_gives_correct_result_base l)
 
-// val maximum_frontier (l:list english_letters) (dim:nat) (i:nat) (j:nat{j <= length l}) : nat
-// let rec maximum_frontier l dim i j =
-//     match j with
-//         | 0 -> 0
-//         | _ -> if compare_frontier l dim i j = true
-//                then j
-//                else maximum_frontier l dim i (j - 1)
+let logical_implication (a:Type) (b:Type)
+  : Lemma (ensures (a <==> b) ==> (~a <==> ~b))
+  = ()
 
-// val append (#a:Type) (m:list a) (n:a) : list a
-// let rec append m n = 
-//     match m with
-//         | [] -> n :: []
-//         | hd :: tl -> hd :: (append tl n)
+let lists_are_not_equal_base (l1:list english_letters) (l2:list english_letters) 
+  : Lemma (requires l1 <> l2)
+          (ensures (length l1 <> length l2) \/ 
+                   (length l1 = length l2 /\ (exists (i:nat{i < length l1 && i < length l2}). index l1 i <> index l2 i)))
+  = compare_lists_not_equal_both_parts l1 l2
 
-// val reverse (#a:Type) (l:list a) : list a
-// let rec reverse l =
-//     match l with
-//         | [] -> []
-//         | hd :: tl -> append (reverse tl) hd
+let lists_are_not_equal_implication (l1:list english_letters) (l2:list english_letters)
+  : Lemma (ensures l1 <> l2 ==> (length l1 <> length l2) \/ 
+                                (length l1 = length l2 /\ (exists (i:nat{i < length l1 && i < length l2}). index l1 i <> index l2 i)))
+  = move_requires (lists_are_not_equal_base l1) l2
 
-// val create_pr (l:list english_letters) (j:nat{j <= length l}) : list int
-// let rec create_pr l j =
-//     match j with 
-//         | 0 -> [-1]
-//         | _ -> (maximum_frontier (first_characters l j) (length (first_characters l j)) 0 (length (first_characters l j))) :: (create_pr l (j - 1))
-               
-// let f : list int = reverse (create_pr pattern (length pattern))
+let compare_first_characters_with_last_characters_false (l:list english_letters) (i:nat{i <= length l})
+  : Lemma (ensures 
+           (let l1 = first_characters l i in
+            let l2 = last_characters l i in 
+            l1 <> l2 ==> (length l1 <> length l2) \/ 
+                         ((length l1 = length l2) /\ (exists (j:nat{j < length l1 && j < length l2}). index l1 j <> index l2 j))))
+  = lists_are_not_equal_implication (first_characters l i) (last_characters l i)
+
+let compare_frontiers_false_gives_correct_result_base (l:list english_letters) (i:nat{i <= length l})
+  : Lemma (ensures 
+           (let l1 = first_characters l i in
+            let l2 = last_characters l i in 
+            compare_frontier l i = false ==> 
+            (length l1 <> length l2) \/
+            ((length l1 = length l2) /\ (exists (j:nat{j < length l1 && j < length l2}). index l1 j <> index l2 j)) \/
+            (l1 = l2 /\ i >= length l)))
+  = compare_first_characters_with_last_characters_false l i
+
+let compare_frontiers_false_gives_correct_result (l:list english_letters) 
+  : Lemma (ensures forall (i:nat{i <= length l}).
+           (let l1 = first_characters l i in
+            let l2 = last_characters l i in 
+            compare_frontier l i = false ==> 
+            (length l1 <> length l2) \/
+            ((length l1 = length l2) /\ (exists (j:nat{j < length l1 && j < length l2}). index l1 j <> index l2 j)) \/
+            (l1 = l2 /\ i >= length l)))
+  = forall_intro (compare_frontiers_false_gives_correct_result_base l)
+
+let maximum (a:int) (b:int)
+  : int 
+  = if a > b 
+    then a 
+    else b 
+
+let maximum_returns_correct_result_base (a:int) (b:int)
+  : Lemma (ensures maximum a b = a ==> a >= b)
+  = ()
+
+let maximum_returns_correct_result ()
+  : Lemma (ensures forall (a:int) (b:int). maximum a b = a ==> a >= b)
+  = forall_intro_2 maximum_returns_correct_result_base
+
+val maximum_frontier (l:list english_letters) (i:nat{i <= length l}) : nat
+let rec maximum_frontier l i =
+    match i with
+        | 0 -> 0
+        | _ -> if compare_frontier l i = true
+               then i
+               else maximum_frontier l (i - 1)
+
+let rec maximum_frontier_max_value (l:list english_letters{l <> []}) (i:nat{i <= length l})
+  : Lemma (ensures maximum_frontier l i < length l)
+  = match i with 
+    | 0 -> ()
+    | _ -> if compare_frontier l i = true 
+           then ()
+           else maximum_frontier_max_value l (i - 1)
+
+let rec maximum_frontier_value (l:list english_letters) (i:nat{i <= length l})
+  : Lemma (ensures maximum_frontier l i <= i)
+  = match i with
+    | 0 -> ()
+    | _ -> if compare_frontier l i = true 
+           then ()
+           else maximum_frontier_value l (i - 1)
+
+//pass
+let rec length_init_list_is_length_list_minus_one (l:list english_letters)
+  : Lemma (requires l <> [])
+          (ensures length (init l) = length l - 1)
+  = match l with 
+    | [el] -> ()
+    | hd :: tl -> length_init_list_is_length_list_minus_one tl
+
+//pass
+let rec maximum_frontier_for_l_and_tail_l (l:list english_letters)
+  : Lemma (requires l <> [])
+          (ensures maximum_frontier l (length l) = maximum_frontier (init l) (length (init l)))
+          (decreases length l)
+  = match l with 
+    | [el] -> ()
+    | _ -> length_init_list_is_length_list_minus_one l;
+           maximum_frontier_for_l_and_tail_l (init l);
+           admit()
+
+let maximum_frontier_zero_no_frontier_for_i (l:list english_letters) (i:nat{i > 0 && i <= length l})
+  : Lemma (requires maximum_frontier l i = 0)
+          (ensures 
+          (let l1 = first_characters l i in 
+           let l2 = last_characters l i in 
+           (length l1 <> length l2) \/ 
+           ((length l1 = length l2) /\ (exists (j:nat{j < length l1 && j < length l2}). index l1 j <> index l2 j)) \/
+           i >= length l))
+           (decreases length l)
+  = compare_frontiers_false_gives_correct_result l
+
+let rec maximum_frontier_zero_for_length_l_and_i_base_general (l:list english_letters) (i:nat{i <= length l}) (j:nat{j <= i})
+  : Lemma (requires maximum_frontier l i = 0)
+          (ensures maximum_frontier l j = 0)
+  = if j = i 
+    then ()
+    else maximum_frontier_zero_for_length_l_and_i_base_general l (i - 1) j
+
+let maximum_frontier_zero_for_length_l_and_i_base (l:list english_letters) (j:nat{j <= length l})
+  : Lemma (requires maximum_frontier l (length l) = 0)
+          (ensures maximum_frontier l j = 0)
+  = maximum_frontier_zero_for_length_l_and_i_base_general l (length l) j
+
+let maximum_frontier_zero_for_length_l_and_i_implication (l:list english_letters) (j:nat{j <= length l})
+  : Lemma (ensures maximum_frontier l (length l) = 0 ==> maximum_frontier l j = 0)
+  = move_requires (maximum_frontier_zero_for_length_l_and_i_base l) j 
+
+let maximum_frontier_zero_for_length_l_and_i (l:list english_letters)
+  : Lemma (ensures forall (j:nat{j <= length l}). maximum_frontier l (length l) = 0 ==> maximum_frontier l j = 0)
+  = forall_intro (maximum_frontier_zero_for_length_l_and_i_implication l)
+
+let maximum_frontier_zero_no_frontier_base (l:list english_letters) (i:nat{i > 0 && i <= length l})
+  : Lemma (requires maximum_frontier l (length l) = 0)
+          (ensures 
+          (let l1 = first_characters l i in 
+           let l2 = last_characters l i in 
+           (length l1 <> length l2) \/ 
+           ((length l1 = length l2) /\ (exists (j:nat{j < length l1 && j < length l2}). index l1 j <> index l2 j)) \/
+           i >= length l))
+           (decreases length l)
+  = maximum_frontier_zero_for_length_l_and_i l;
+    maximum_frontier_zero_no_frontier_for_i l i 
+
+let maximum_frontier_zero_no_frontier_implication (l:list english_letters) (i:nat{i > 0 && i <= length l})
+  : Lemma (ensures maximum_frontier l (length l) = 0 ==>
+           (let l1 = first_characters l i in 
+           let l2 = last_characters l i in 
+           (length l1 <> length l2) \/ 
+           ((length l1 = length l2) /\ (exists (j:nat{j < length l1 && j < length l2}). index l1 j <> index l2 j)) \/
+           i >= length l))
+  = move_requires (maximum_frontier_zero_no_frontier_base l) i 
+
+let maximum_frontier_zero_no_frontier (l:list english_letters)
+  : Lemma (ensures forall (i:nat{i > 0 && i <= length l}). maximum_frontier l (length l) = 0 ==>
+           (let l1 = first_characters l i in 
+           let l2 = last_characters l i in 
+           (length l1 <> length l2) \/ 
+           (length l1 = length l2) \/ (exists (j:nat{j < length l1 && j < length l2}). index l1 j <> index l2 j) \/
+           i >= length l))
+  = forall_intro (maximum_frontier_zero_no_frontier_implication l)
+
+let rec maximum_frontier_i_then_compare_frontier_true (l:list english_letters) (i:nat{i > 0 && i <= length l})
+  : Lemma (ensures maximum_frontier l i = i ==> compare_frontier l i = true)
+  = match i with 
+    | 1 -> ()
+    | _ -> if compare_frontier l i = true 
+           then ()
+           else (
+            assert(maximum_frontier l i = maximum_frontier l (i - 1));
+            maximum_frontier_value l (i - 1);
+            assert(maximum_frontier l (i - 1) <= i - 1);
+            maximum_frontier_i_then_compare_frontier_true l (i - 1)
+           )
+
+let rec maximum_frontier_not_zero_has_compare_frontier_true (l:list english_letters) (i:nat{i > 0 && i <= length l})
+  : Lemma (requires maximum_frontier l i <> 0 && maximum_frontier l i <= length l)
+          (ensures 
+          (let j = maximum_frontier l i in 
+           compare_frontier l j = true))
+  = let j = maximum_frontier l i in 
+    if j = i 
+    then maximum_frontier_i_then_compare_frontier_true l i
+    else maximum_frontier_not_zero_has_compare_frontier_true l (i - 1)
+
+let maximum_frontier_not_zero_equal_lists (l:list english_letters) (i:nat{i > 0 && i <= length l})
+  : Lemma (requires maximum_frontier l i <> 0 && maximum_frontier l i <= length l)
+          (ensures 
+          (let x = maximum_frontier l i in 
+           let l1 = first_characters l x in 
+           let l2 = last_characters l x in 
+           l1 = l2 && x < length l))
+  = maximum_frontier_not_zero_has_compare_frontier_true l i;
+    compare_frontiers_true_gives_correct_result l
+
+let maximum_frontier_not_i_then_compare_frontier_false (l:list english_letters) (i:nat{i <= length l})
+  : Lemma (ensures maximum_frontier l i <> i ==> compare_frontier l i = false)
+  = ()
+
+let rec maximum_frontier_i_then_compare_frontier_false_if_greater_than_i (l:list english_letters) (i:nat{i <= length l})
+                                                                         (i':nat)
+  : Lemma (requires i' > maximum_frontier l i && i' <= i)
+          (ensures compare_frontier l i' = false)
+  = if i = i'
+    then maximum_frontier_not_i_then_compare_frontier_false l i'
+    else maximum_frontier_i_then_compare_frontier_false_if_greater_than_i l (i - 1) i'
+
+let maximum_frontier_not_zero_not_equal_rest_of_the_lists_base (l:list english_letters) (i:nat{i > 0 && i <= length l})
+                                                               (i':nat{i' > maximum_frontier l i && i' <= i && i' < length l})
+  : Lemma (ensures 
+          (let l1 = first_characters l i' in 
+           let l2 = last_characters l i' in 
+           l1 <> l2))
+  = maximum_frontier_i_then_compare_frontier_false_if_greater_than_i l i i';
+    compare_frontiers_false_gives_correct_result l 
+
+let maximum_frontier_not_zero_not_equal_rest_of_the_lists (l:list english_letters) (i:nat{i > 0 && i <= length l})
+  : Lemma (ensures forall (i':nat{i' > maximum_frontier l i && i' <= i && i' < length l}).
+          (let l1 = first_characters l i' in 
+           let l2 = last_characters l i' in 
+           l1 <> l2))
+  = forall_intro (maximum_frontier_not_zero_not_equal_rest_of_the_lists_base l i)
+
+let maximum_frontier_not_zero_correct_value (l:list english_letters) (i:nat{i > 0 && i <= length l})
+  : Lemma (requires maximum_frontier l i <> 0 && maximum_frontier l i <= length l)
+          (ensures 
+          (let x = maximum_frontier l i in 
+           let l1 = first_characters l x in 
+           let l2 = last_characters l x in 
+           l1 = l2 /\ 
+           (forall (i':nat{i' > maximum_frontier l i && i' < i && i' < length l}). 
+            let l3 = first_characters l i' in 
+            let l4 = last_characters l i' in 
+            l3 <> l4)))
+  = maximum_frontier_not_zero_equal_lists l i;
+    maximum_frontier_not_zero_not_equal_rest_of_the_lists l i
+
+// let rev_stores_correct_indices (#a:eqtype) (l:list a) (i:nat{i < length l})
+//   : Lemma (requires length l = length (rev l))
+//           (ensures index l i = index (rev l) (length l - 1 - i))
+//   = assert(rev l = rev_acc l []);
+//     assert(rev_acc l [] = rev_acc (tail l) [hd l])
+    // assert(rev_acc (tail l) [hd l] = rev_acc [] ((last l) :: (init l)))
+
+// let rec tail_rev_is_init_l (#a:eqtype) (l:list a{l <> []})
+//   : Lemma (requires length l = length (rev l))
+//           (ensures tail (rev l) = rev (init l))
+//   = match l with 
+//     | [el] -> ()
+//     | fst :: ot -> rev_length ot; 
+//                    tail_rev_is_init_l ot 
+
+let rec create_pr (l:list english_letters) (i:nat{i > 0 && i <= length l})
+  : Tot (list int) 
+  (decreases length l - i)
+  = if i = length l 
+    then [maximum_frontier (first_characters l i) (length (first_characters l i))]
+    else (maximum_frontier (first_characters l i) (length (first_characters l i))) :: (create_pr l (i + 1))
+
+let rec create_pr_has_same_length_as_initial_list_general (l:list english_letters) (i:nat{i > 0 && i <= length l})
+  : Lemma (ensures
+          (let l' = create_pr l i in 
+           length l' = length l + 1 - i))
+          (decreases length l - i)
+  = if i = length l 
+    then () 
+    else create_pr_has_same_length_as_initial_list_general l (i + 1)
+
+let create_pr_has_same_length_as_initial_list_base (l:list english_letters{l <> []})
+  : Lemma (ensures
+          (let l' = create_pr l 1 in 
+           length l' = length l))
+  = create_pr_has_same_length_as_initial_list_general l 1
+
+let create_pr_has_same_length_as_initial_list ()
+  : Lemma (ensures forall (l:list english_letters{l <> []}).
+          (let l' = create_pr l 1 in 
+           length l' = length l))
+  = forall_intro (create_pr_has_same_length_as_initial_list_base)
+
+let length_equal_then_length_tail_equal (l1:list english_letters{l1 <> []}) (l2:list english_letters{l2 <> []})
+  : Lemma (requires length l1 = length l2)
+          (ensures length (tail l1) = length (tail l2))
+  = ()
+
+let create_pr_tail (l:list english_letters{l <> []}) (i:nat{i > 0 && i < length l})
+  : Lemma (ensures create_pr l (i + 1) = tail (create_pr l i))
+  = ()
+
+let rec create_pr_values_are_in_correct_index_base (l:list english_letters{l <> []}) 
+                                                   (i:nat{i > 0 && i <= length l}) (j:nat{j < length (create_pr l i)})
+  : Lemma (ensures 
+          (let l' = create_pr l i in 
+           index l' j >= 0 && index l' j < i + j))
+           (decreases length l - i)
+  = if j = 0
+    then (
+      length_first_characters_i_is_i l i;
+      first_characters_stores_indices_correctly l i;
+      maximum_frontier_max_value (first_characters l i) i
+    )
+    else (
+      assert(index (create_pr l i) j = index (tail (create_pr l i)) (j - 1));
+        assert(index (create_pr l i) j = index (create_pr l (i + 1)) (j - 1));
+        create_pr_has_same_length_as_initial_list_general l i;
+        create_pr_has_same_length_as_initial_list_general l (i + 1);
+        assert(j < length (create_pr l i));
+        assert(j < length l + 1 - i);
+        assert(j - 1 < length l - i);
+        create_pr_values_are_in_correct_index_base l (i + 1) (j - 1);
+        assert(index (create_pr l (i + 1)) (j - 1) >= 0 && index (create_pr l (i + 1)) (j - 1) < (i + j))
+    )
+
+let create_pr_values_are_in_correct_index_forall_j (l:list english_letters{l <> []}) (i:nat{i > 0 && i <= length l})
+  : Lemma (ensures forall (j:nat{j < length (create_pr l i)}). 
+          (let l' = create_pr l i in 
+           index l' j >= 0 && index l' j < i + j))
+  = forall_intro (create_pr_values_are_in_correct_index_base l i) 
+
+let create_pr_values_are_in_correct_index (l:list english_letters{l <> []})
+  : Lemma (ensures forall (i:nat{i > 0 && i <= length l}) (j:nat{j < length (create_pr l i)}). 
+          (let l' = create_pr l i in 
+           index l' j >= 0 && index l' j < i + j))
+  = forall_intro (create_pr_values_are_in_correct_index_forall_j l)
+
+// let rec go_through_rev_create_pr (l:list english_letters{l <> []}) 
+//                                  (i:nat{i > 0 && i <= length l}) (j:nat{j < length (create_pr l i)})
+//   : Lemma (requires length (create_pr l i) = length (rev (create_pr l i)) && length (create_pr l i) = length l + 1 - i)
+//           (ensures 
+//           (let l' = rev (create_pr l i) in 
+//            index l' j = maximum_frontier (first_characters l (length l - j)) (length (first_characters l (length l - j)))))
+//   = if j = 0 
+//     then admit()
+//     else go_through_rev_create_pr l i (j - 1)
+
+// let rec rev_create_pr_values_are_in_correct_index_base (l:list english_letters{l <> []}) 
+//                                                        (i:nat{i > 0 && i <= length l}) (j:nat{j < length (create_pr l i)})
+//   : Lemma (requires length (create_pr l i) = length (rev (create_pr l i)))
+//           (ensures 
+//           (let l' = rev (create_pr l i) in 
+//            index l' j >= 0 && index l' j < i + j))
+//           (decreases length l - i)
+  // = if j = 0
+  //   then (
+  //     rev_mem (create_pr l i) (index (create_pr l i) j);
+  //     length_first_characters_i_is_i l i;
+  //     first_characters_stores_indices_correctly l i;
+  //     maximum_frontier_max_value (first_characters l i) i;
+  //     admit()
+  //   )
+  //   else (
+  //     rev_length (create_pr l (i + 1));
+  //     tail_rev_l_is_rev_tl (create_pr l i);
+  //     rev_create_pr_values_are_in_correct_index_base l (i + 1) (j - 1)
+  //   )
+
+let rec create_pr_gives_correct_result_base (l:list english_letters{l <> []}) 
+                                            (i:nat{i > 0 && i <= length l}) 
+                                            (j:nat{j < length (create_pr l i)})
+  : Lemma (requires length (create_pr l i) = length l + 1 - i)
+          (ensures
+          (let l' = create_pr l i in 
+           let x = index l' j in 
+           x = maximum_frontier (first_characters l (i + j)) (length (first_characters l (i + j)))))
+          (decreases j)
+  = if j = 0 
+    then ()
+    else (
+      create_pr_has_same_length_as_initial_list_general l (i + 1);
+      assert(length (create_pr l (i + 1)) = length l + 1 - (i + 1));
+      assert(create_pr l i = (maximum_frontier (first_characters l i) (length (first_characters l i))) :: (create_pr l (i + 1)));
+      assert(index (create_pr l i) j = index (tail (create_pr l i)) (j - 1));
+      assert(index (tail (create_pr l i)) (j - 1) = index (create_pr l (i + 1)) (j - 1));
+      assert(j < length l + 1 - i);
+      assert(j + i < length l + 1);
+      assert(j + i <= length l);
+      assert(j - 1 < length l + 1 - (i + 1));
+      assert(j - 1 < length l - i);
+      assert(j + i < length l + 1);
+      assert(j + i <= length l);
+      create_pr_gives_correct_result_base l (i + 1) (j - 1)
+    )
+
+let create_pr_gives_correct_result_implication (l:list english_letters{l <> []}) 
+                                               (i:nat{i > 0 && i <= length l}) 
+                                               (j:nat{j < length (create_pr l i)})
+  : Lemma (ensures length (create_pr l i) = length l + 1 - i ==> 
+          (let l' = create_pr l i in 
+           let x = index l' j in 
+           x = maximum_frontier (first_characters l (i + j)) (length (first_characters l (i + j)))))
+  = create_pr_has_same_length_as_initial_list_general l i;
+    move_requires (create_pr_gives_correct_result_base l i) j 
+
+let create_pr_gives_correct_result_forall_j (l:list english_letters{l <> []}) 
+                                                        (i:nat{i > 0 && i <= length l}) 
+  : Lemma (ensures forall (j:nat{j < length (create_pr l i)}). length (create_pr l i) = length l + 1 - i ==> 
+          (let l' = create_pr l i in 
+           let x = index l' j in 
+           x = maximum_frontier (first_characters l (i + j)) (length (first_characters l (i + j)))))
+  = forall_intro (create_pr_gives_correct_result_implication l i)
+
+let create_pr_gives_correct_result (l:list english_letters{l <> []}) 
+  : Lemma (ensures forall (i:nat{i > 0 && i <= length l})  (j:nat{j < length (create_pr l i)}). 
+           length (create_pr l i) = length l + 1 - i ==> 
+          (let l' = create_pr l i in 
+           let x = index l' j in 
+           x = maximum_frontier (first_characters l (i + j)) (length (first_characters l (i + j)))))
+  = forall_intro (create_pr_gives_correct_result_forall_j l)
+
+let f : list int = create_pr pattern 1
+
+let create_pr_has_same_length_as_initial_list_for_pattern ()
+  : Lemma (ensures length f = length pattern)
+  = create_pr_has_same_length_as_initial_list_base pattern
+
+let create_pr_values_are_in_correct_index_for_pattern ()
+  : Lemma (ensures forall (j:nat{j < length f}). 
+           index f j >= 0 && index f j < 1 + j)
+  = create_pr_values_are_in_correct_index_forall_j pattern 1
+
+let create_pr_gives_correct_result_for_pattern ()
+  : Lemma (ensures forall (j:nat{j < length f}). length f = length pattern ==> 
+          (let x = index f j in 
+           x = maximum_frontier (first_characters pattern (1 + j)) (length (first_characters pattern (1 + j)))))
+  = create_pr_gives_correct_result_forall_j pattern 1
 
 // val give_value (f:list int) (nr:int) (i:nat{i >= 0}) : int
 // let rec give_value f nr i =
@@ -347,31 +714,425 @@ let compare_frontiers_true_gives_correct_result (l:list english_letters) (i:nat{
 //                     then hd
 //                     else give_value tl nr (i + 1)
 
-// val create_gs (f:list int) (m:nat) (i:nat{i >= 0}) : list int
-// let rec create_gs f m i =
-//     match i with
-//         | 0 -> [(give_value f m 0) - m]
-//         | _ -> ((give_value f m 0) - m + i) :: (create_gs f m (i - 1))
-        
-// let gs : list int = reverse (create_gs f (length pattern) ((length pattern) - 1))
- 
-// let r : list english_letters = reverse pattern
-// let g : list int = reverse (create_pr r (length r)) 
-// let h : list int = reverse g
+let rec substring (#a:eqtype) (l:list a) (i:nat{i < length l}) (j:nat{j >= i && j < length l})
+  : Tot (list a) 
+  (decreases length l - i)
+  = if i = j 
+    then [index l i]
+    else (index l i) :: substring l (i + 1) j
 
-// val change_value (l:list int) (m:int) (n:int) (i:nat{i >= 0}) : list int
-// let rec change_value l m n i : Tot (list int) (decreases l) =
-//     match l with
-//         | [] -> []
-//         | hd :: tl -> if i = m
-//                       then n :: change_value tl m n (i + 1)
-//                       else hd :: change_value tl m n (i + 1)
-                      
+let rec substring_list_length (#a:eqtype) (l:list a) (i:nat{i < length l}) (j:nat{j >= i && j < length l})
+  : Lemma (ensures length (substring l i j) = j - i + 1)
+  (decreases length l - i)
+  = if i = j 
+    then ()
+    else substring_list_length l (i + 1) j
+
+let rec substring_stores_correct_values_base (#a:eqtype) (l:list a) (i:nat{i < length l}) (j:nat{j >= i && j < length l}) (k:nat{k >= i && k <= j})
+  : Lemma (requires k - i < length (substring l i j))
+          (ensures 
+          (let l' = substring l i j in 
+           index l k = index l' (k - i)))
+          (decreases length l - i)
+  = if i = k 
+    then ()
+    else substring_stores_correct_values_base l (i + 1) j k
+
+let substring_stores_correct_values_implication (#a:eqtype) (l:list a) (i:nat{i < length l}) (j:nat{j >= i && j < length l}) (k:nat{k >= i && k <= j})
+  : Lemma (ensures 
+          (let l' = substring l i j in 
+           k - i < length (substring l i j) ==> index l k = index l' (k - i)))
+  = substring_list_length l i j;
+    move_requires (substring_stores_correct_values_base l i j) k
+
+let substring_stores_correct_values (#a:eqtype) (l:list a) (i:nat{i < length l}) (j:nat{j >= i && j < length l}) 
+  : Lemma (ensures forall (k:nat{k >= i && k <= j}).
+          (let l' = substring l i j in 
+           k - i < length (substring l i j) ==> index l k = index l' (k - i)))
+  = forall_intro (substring_stores_correct_values_implication l i j)
+
+let rec create_gs (l:list english_letters) (i:nat{i <= length l}) 
+  : Tot (list int) 
+  (decreases length l - i)
+  = if i = length l
+    then [] 
+    else (
+      create_pr_has_same_length_as_initial_list_base l;
+      (index (create_pr l 1) (length l - 1) - (length l - i)) :: (create_gs l (i + 1))
+    )
+
+let rec create_gs_length_is_l_length_general (l:list english_letters) (i:nat{i <= length l})  
+  : Lemma (ensures 
+          (let l' = create_gs l i in 
+           length l' = length l - i))
+          (decreases length l - i)
+  = if i = length l 
+    then ()
+    else create_gs_length_is_l_length_general l (i + 1)
+
+let create_gs_length_is_l_length_base (l:list english_letters)
+  : Lemma (ensures 
+          (let l' = create_gs l 0 in 
+           length l' = length l))
+  = create_gs_length_is_l_length_general l 0
+
+let create_gs_length_is_l_length ()
+  : Lemma (ensures forall (l:list english_letters).
+          (let l' = create_gs l 0 in 
+           length l' = length l))
+  = forall_intro create_gs_length_is_l_length_base
+
+let rec create_gs_values_general (l:list english_letters) (i:nat{i < length l}) (j:nat{j < length l - i})
+  : Lemma (requires length (create_pr l 1) = length l && length (create_gs l i) = length l - i)
+          (ensures 
+          (let l' = create_gs l i in 
+           index l' j = index (create_pr l 1) (length l - 1) - (length l - (i + j))))
+          (decreases length l - i)
+  = if j = 0 
+    then ()
+    else (
+      create_pr_has_same_length_as_initial_list_base l;
+      create_gs_length_is_l_length_general l (i + 1);
+      assert(create_gs l i = (index (create_pr l 1) (length l - 1) - (length l - i)) :: (create_gs l (i + 1)));
+      assert(index (create_gs l i ) j = index (tail (create_gs l i)) (j - 1));
+      assert(tail (create_gs l i) = create_gs l (i + 1));
+      assert(index (create_gs l i ) j = index (create_gs l (i + 1)) (j - 1));
+      create_gs_values_general l (i + 1) (j - 1)
+    )
+        
+let create_gs_values_base (l:list english_letters) (i:nat{i < length l}) (j:nat{j < length l - i})
+  : Lemma (ensures length (create_pr l 1) = length l && length (create_gs l i) = length l - i ==> 
+          (let l' = create_gs l i in 
+           index l' j = index (create_pr l 1) (length l - 1) - (length l - (i + j))))
+  = create_pr_has_same_length_as_initial_list_base l;
+    create_gs_length_is_l_length_general l i;
+    move_requires (create_gs_values_general l i) j
+
+let create_gs_values_forall_j (l:list english_letters) (i:nat{i < length l})
+  : Lemma (ensures forall (j:nat{j < length l - i}).
+           length (create_pr l 1) = length l && length (create_gs l i) = length l - i ==> 
+          (let l' = create_gs l i in 
+           index l' j = index (create_pr l 1) (length l - 1) - (length l - (i + j))))
+  = forall_intro (create_gs_values_base l i)
+
+let create_gs_values (l:list english_letters)
+  : Lemma (ensures forall (i:nat{i < length l}) (j:nat{j < length l - i}).
+           length (create_pr l 1) = length l && length (create_gs l i) = length l - i ==> 
+          (let l' = create_gs l i in 
+           index l' j = index (create_pr l 1) (length l - 1) - (length l - (i + j))))
+  = forall_intro (create_gs_values_forall_j l)
+
+let rec append (#a:eqtype) (l1:list a) (l2:list a)
+  : list a 
+  = match l1 with 
+    | [] -> l2 
+    | hd :: tl -> hd :: (append tl l2)
+
+let rec append_length (#a:eqtype) (l1:list a) (l2:list a)
+  : Lemma (ensures length (append l1 l2) = length l1 + length l2)
+  = match l1 with 
+    | [] -> ()
+    | hd :: tl -> append_length tl l2 
+
+let rec append_indices_from_first_list_are_stored_correctly_base (#a:eqtype) (l1:list a) (l2:list a) (i:nat{i < length l1})
+  : Lemma (requires length (append l1 l2) = length l1 + length l2)
+          (ensures index (append l1 l2) i = index l1 i)
+  = if i = 0 
+    then ()
+    else append_indices_from_first_list_are_stored_correctly_base (tail l1) l2 (i - 1)
+
+let append_indices_from_first_list_are_stored_correctly_implication (#a:eqtype) (l1:list a) (l2:list a) (i:nat{i < length l1})
+  : Lemma (ensures length (append l1 l2) = length l1 + length l2 ==> index (append l1 l2) i = index l1 i)
+  = append_length l1 l2;
+    move_requires (append_indices_from_first_list_are_stored_correctly_base l1 l2) i
+
+let append_indices_from_first_list_are_stored_correctly (#a:eqtype) (l1:list a) (l2:list a)
+  : Lemma (ensures forall (i:nat{i < length l1}). length (append l1 l2) = length l1 + length l2 ==> index (append l1 l2) i = index l1 i)
+  = forall_intro (append_indices_from_first_list_are_stored_correctly_implication l1 l2)
+
+let rec append_indices_from_second_list_are_stored_correctly_base (#a:eqtype) (l1:list a) (l2:list a) 
+                                                                  (i:nat{i >= length l1 && i < length l1 + length l2})
+  : Lemma (requires length (append l1 l2) = length l1 + length l2)
+          (ensures index (append l1 l2) i = index l2 (i - length l1))
+  = if length l1 = 0 
+    then ()
+    else append_indices_from_second_list_are_stored_correctly_base (tail l1) l2 (i - 1)
+
+let append_indices_from_second_list_are_stored_correctly_implication (#a:eqtype) (l1:list a) (l2:list a) 
+                                                                     (i:nat{i >= length l1 && i < length l1 + length l2})
+  : Lemma (ensures length (append l1 l2) = length l1 + length l2 ==> index (append l1 l2) i = index l2 (i - length l1))
+  = append_length l1 l2;
+    move_requires (append_indices_from_second_list_are_stored_correctly_base l1 l2) i
+
+let append_indices_from_second_list_are_stored_correctly (#a:eqtype) (l1:list a) (l2:list a) 
+  : Lemma (ensures forall (i:nat{i >= length l1 && i < length l1 + length l2}). 
+           length (append l1 l2) = length l1 + length l2 ==> index (append l1 l2) i = index l2 (i - length l1))
+  = forall_intro (append_indices_from_second_list_are_stored_correctly_implication l1 l2)
+
+let append_indices_are_stored_correctly (#a:eqtype) (l1:list a) (l2:list a) 
+  : Lemma (ensures forall (i:nat{i < length l1}) (j:nat{j >= length l1 && j < length l1 + length l2}). 
+           length (append l1 l2) = length l1 + length l2 ==> 
+           index (append l1 l2) i = index l1 i && index (append l1 l2) j = index l2 (j - length l1))
+  = append_indices_from_first_list_are_stored_correctly l1 l2;
+    append_indices_from_second_list_are_stored_correctly l1 l2
+
+let rec reverse (#a:eqtype) (l:list a)
+  : list a 
+  = match l with 
+    | [] -> []
+    | hd :: tl -> append (reverse tl) [hd] 
+
+let rec reverse_length_is_l_length (#a:eqtype) (l:list a)
+  : Lemma (ensures length l = length (reverse l))
+  = match l with 
+    | [] -> ()
+    | hd :: tl -> reverse_length_is_l_length tl;
+                  append_length (reverse tl) [hd]
+
+let rec last_from_append_is_init (#a:eqtype) (l:list a) (el:a)
+  : Lemma (ensures init (append l [el]) = l)
+  = match l with 
+    | [] -> ()
+    | hd :: tl -> last_from_append_is_init tl el
+
+//repeated
+let rec length_init_list (#a:eqtype) (l:list a)
+  : Lemma (requires l <> [])
+          (ensures length (init l) = length l - 1)
+  = match l with 
+    | [el] -> ()
+    | hd :: tl -> length_init_list tl
+
+let rec init_l_has_same_indices_except_last_base (#a:eqtype) (l:list a{length l > 1}) (i:nat{i < length l - 1})
+  : Lemma (requires length (init l) = length l - 1)
+          (ensures index l i = index (init l) i)
+  = if i = 0
+    then ()
+    else (
+      length_init_list (tail l);
+      init_l_has_same_indices_except_last_base (tail l) (i - 1)
+    )
+
+let init_l_has_same_indices_except_last_implication (#a:eqtype) (l:list a{length l > 1}) (i:nat{i < length l - 1})
+  : Lemma (ensures length (init l) = length l - 1 ==> index l i = index (init l) i)
+  = length_init_list l;
+    move_requires (init_l_has_same_indices_except_last_base l) i
+
+let init_l_has_same_indices_except_last (#a:eqtype) (l:list a{length l > 1})
+  : Lemma (ensures forall (i:nat{i < length l - 1}). length (init l) = length l - 1 ==> index l i = index (init l) i)
+  = forall_intro (init_l_has_same_indices_except_last_implication l)
+
+let rec reverse_stores_correct_values_base (#a:eqtype) (l:list a) (i:nat{i < length l})
+  : Lemma (requires length l = length (reverse l))
+          (ensures index l i = index (reverse l) (length l - 1 - i))
+  = if i = 0 
+    then (
+      append_length (reverse (tail l)) [hd l];
+      append_indices_from_second_list_are_stored_correctly_base (reverse (tail l)) [hd l] (length l - 1)
+    )
+    else (
+      reverse_length_is_l_length (tail l);
+      reverse_stores_correct_values_base (tail l) (i - 1);
+      assert(reverse l = append (reverse (tail l)) [hd l]);
+      last_from_append_is_init (reverse (tail l)) (hd l);
+      assert(init (reverse l) = init (append (reverse (tail l)) [hd l]));
+      assert(init (append (reverse (tail l)) [hd l]) = (reverse (tail l)));
+      assert(length (tail l) - 1 - (i - 1) = length l - 1 - i);
+      assert(reverse (tail l) = init (reverse l));
+      init_l_has_same_indices_except_last (reverse l);
+      assert(index (reverse l) (length l - 1 - i) = index (init (reverse l)) (length (tail l) - 1 - (i - 1)))
+    )
+
+let reverse_stores_correct_values_implication (#a:eqtype) (l:list a) (i:nat{i < length l})
+  : Lemma (ensures length l = length (reverse l) ==> index l i = index (reverse l) (length l - 1 - i))
+  = reverse_length_is_l_length l;
+    move_requires (reverse_stores_correct_values_base l) i
+
+let reverse_stores_correct_values (#a:eqtype) (l:list a)
+  : Lemma (ensures forall (i:nat{i < length l}). length l = length (reverse l) ==> index l i = index (reverse l) (length l - 1 - i))
+  = forall_intro (reverse_stores_correct_values_implication l)
+
+let reverse_stores_correct_values_other (#a:eqtype) (l:list a)
+  : Lemma (ensures forall (i:nat{i < length l}). length l = length (reverse l) ==> index l (length l - 1 - i) = index (reverse l) i)
+  = reverse_stores_correct_values l
+
+let gs : list int = create_gs pattern 0
+ 
+let create_gs_length_is_l_length_for_gs ()
+  : Lemma (ensures length gs = length pattern)
+  = create_gs_length_is_l_length_base pattern
+
+let create_gs_values_for_gs ()
+  : Lemma (ensures forall (j:nat{j < length pattern}).
+           length f = length pattern && length gs = length pattern ==>
+           index gs j = index f (length pattern - 1) - (length pattern - j))
+  = create_gs_values_forall_j pattern 0 
+
+let r : (l:list english_letters{l <> []}) 
+  = reverse pattern
+
+let r_has_same_length_as_pattern ()
+  : Lemma (ensures length r = length pattern)
+  = reverse_length_is_l_length pattern
+
+let r_has_correct_indices_stored ()
+  : Lemma (ensures forall (i:nat{i < length pattern}). length pattern = length r ==> index pattern i = index r (length pattern - 1 - i))
+  = reverse_stores_correct_values pattern
+
+let g : (l:list int{l <> []}) 
+    = create_pr r 1
+
+let g_has_same_length_as_r ()
+  : Lemma (ensures length g = length r)
+  = create_pr_has_same_length_as_initial_list_base r
+
+let create_pr_values_are_in_correct_index_for_g ()
+  : Lemma (ensures forall (j:nat{j < length g}). index g j >= 0 && index g j < 1 + j)
+  = create_pr_values_are_in_correct_index_forall_j r 1
+
+let create_pr_gives_correct_result_for_g ()
+  : Lemma (ensures forall (j:nat{j < length g}). length g = length r ==> 
+          (let x = index g j in 
+           x = maximum_frontier (first_characters r (1 + j)) (length (first_characters r (1 + j)))))
+  = create_pr_gives_correct_result_forall_j r 1
+
+let h : (l:list int{l <> []}) 
+  = reverse g
+
+let h_has_same_length_as_g ()
+  : Lemma (ensures length h = length g)
+  = reverse_length_is_l_length g 
+
+let h_has_correct_indices_stored ()
+  : Lemma (ensures forall (i:nat{i < length g}). length g = length h ==> index g i = index h (length g - 1 - i))
+  = reverse_stores_correct_values g
+
+let h_has_correct_indices_stored_other ()
+  : Lemma (ensures forall (i:nat{i < length g}). length g = length h ==> index h i = index g (length g - 1 - i))
+  = reverse_stores_correct_values_other g
+
+let first_characters_l_is_last_characters_reverse_l_base (l:list english_letters{l <> []}) (i:nat{i > 0 && i <= length l})
+  : Lemma (requires length l = length (reverse l))
+          (ensures first_characters l i = reverse (last_characters (reverse l) i))
+  = reverse_length_is_l_length l;
+    length_first_characters_i_is_i l i;
+    length_last_characters_i_is_i (reverse l) i;
+    reverse_length_is_l_length (last_characters (reverse l) i);
+    assert(length (last_characters (reverse l) i) = i);
+    assert(length (reverse (last_characters (reverse l) i)) = i);
+    assert(length (first_characters l i) = length (reverse (last_characters (reverse l) i)));
+    reverse_stores_correct_values l;
+    assert(forall (j:nat{j < length l}). index l j = index (reverse l) (length l - 1 - j));
+    first_characters_stores_indices_correctly l i;
+    assert(forall (j:nat{j < i}). index (first_characters l i) j = index l j);
+    assert(forall (j:nat{j < i}). index (first_characters l i) j = index (reverse l) (length l - 1 - j));
+    last_characters_stores_indices_correctly (reverse l) i;
+    assert(forall (j:nat{j < i}). index (last_characters (reverse l) i) j = index (reverse l) (length l - i + j));
+    reverse_stores_correct_values_other (last_characters (reverse l) i);
+    assert(forall (j:nat{j < i}). index (reverse (last_characters (reverse l) i)) j = index (last_characters (reverse l) i) (i - 1 - j));
+    compare_lists_equal_both_parts (first_characters l i) (reverse (last_characters (reverse l) i))
+
+let first_characters_l_is_last_characters_reverse_l_implication (l:list english_letters{l <> []}) (i:nat{i > 0 && i <= length l})
+  : Lemma (ensures length l = length (reverse l) ==> first_characters l i = reverse (last_characters (reverse l) i))
+  = reverse_length_is_l_length l;
+    move_requires (first_characters_l_is_last_characters_reverse_l_base l) i
+
+let first_characters_l_is_last_characters_reverse_l (l:list english_letters{l <> []}) 
+  : Lemma (ensures forall (i:nat{i > 0 && i <= length l}). 
+           length l = length (reverse l) ==> first_characters l i = reverse (last_characters (reverse l) i))
+  = forall_intro (first_characters_l_is_last_characters_reverse_l_implication l)
+
+
+
+// let rec change_value (l:list int) (i:nat) (j:nat) (x:int) 
+//   : list int 
+//   = match l with
+//     | [] -> []
+//     | hd :: tl -> if i = j
+//                   then x :: change_value tl (i + 1) j x 
+//                   else hd :: change_value tl (i + 1) j x
+
+let rec change_value (l:list int) (i:nat{i < length l}) (x:int)
+  : list int 
+  = match l with 
+    | [] -> []
+    | hd :: tl -> if i = 0 
+                  then x :: tl 
+                  else hd :: (change_value tl (i - 1) x)
+
+let rec change_value_length_is_l_length_base (l:list int) (i:nat{i < length l}) (x:int) 
+  : Lemma (ensures length (change_value l i x) = length l)
+  = match l with 
+    | [] -> ()
+    | hd :: tl -> if i = 0 
+                  then ()
+                  else change_value_length_is_l_length_base tl (i - 1) x
+
+let change_value_length_is_l_length (l:list int)
+  : Lemma (ensures forall (i:nat{i < length l}) (x:int). length (change_value l i x) = length l)
+  = forall_intro_2 (change_value_length_is_l_length_base l)
+
+let rec change_value_has_correct_item_changed (l:list int) (i:nat{i < length l}) (x:int) 
+  : Lemma (requires length l = length (change_value l i x))
+          (ensures 
+          (let l' = change_value l i x in 
+           index l' i = x))
+  = if i = 0 
+    then ()
+    else change_value_has_correct_item_changed (tail l) (i - 1) x
+
+let rec change_value_has_the_same_items_base (l:list int) (i:nat{i < length l}) (x:int) 
+                                             (j:nat{j < length l && j < length (change_value l i x) && j <> i})
+  : Lemma (requires length l = length (change_value l i x))
+          (ensures 
+          (let l' = change_value l i x in 
+           index l' j = index l j))
+  = if i = 0 
+    then ()
+    else (
+      if j = 0 
+      then ()
+      else change_value_has_the_same_items_base (tail l) (i - 1) x (j - 1)
+    )
+
+let change_value_has_the_same_items_implication (l:list int) (i:nat{i < length l}) (x:int) 
+                                                (j:nat{j < length l && j < length (change_value l i x) && j <> i})
+  : Lemma (ensures 
+          (let l' = change_value l i x in 
+           length l = length l' ==> index l' j = index l j))
+  = move_requires (change_value_has_the_same_items_base l i x) j
+
+let change_value_has_the_same_items (l:list int) (i:nat{i < length l}) (x:int) 
+  : Lemma (ensures 
+          (let l' = change_value l i x in forall (j:nat{j < length l && j < length (change_value l i x) && j <> i}).
+           length l = length l' ==> index l' j = index l j))
+  = forall_intro (change_value_has_the_same_items_implication l i x)
+
+let change_value_has_correct_result (l:list int) (i:nat{i < length l}) (x:int) 
+  : Lemma (requires length l = length (change_value l i x))
+          (ensures 
+          (let l' = change_value l i x in forall (j:nat{j < length l && j < length (change_value l i x) && j <> i}).
+           index l' i = x && index l' j = index l j))
+  = change_value_has_correct_item_changed l i x;
+    change_value_has_the_same_items l i x
+
 // val update_gs (gs:list int) (h:list int) (i:int{i >= 0}) (dim:nat) : Tot (list int) (decreases i)
 // let rec update_gs gs h i dim =
 //     match i with
 //         | 0 -> gs
 //         | _ -> update_gs (change_value gs (dim - (give_value h (dim - i) 0)) (dim - i) 0) h (i - 1) dim
+
+// let rec update_gs (l:list int) (gs:list int{length gs = length l}) 
+//                   (h:list int{length h = length l}) (i:nat{i <= length l})
+//   : Tot (list int)
+//     (decreases length l - i)
+//   = 
+//     if i = length l 
+//     then gs
+//     else let len = index h i in 
+//          let gs' = change_value gs (length l - len) i in 
+//          change_value_length_is_l_length gs;
+//          update_gs l gs' h (i + 1)
 
 // let final_gs : list int = append (update_gs gs h (length pattern) (length pattern)) ((length pattern) - 1)
 
@@ -398,13 +1159,13 @@ let compare_frontiers_true_gives_correct_result (l:list english_letters) (i:nat{
 //                   else boyer_moore (k - 1) i m n t p bc gs alphabet
 
 //conversion functions, print and main
-let rec belongs (t:list english_letters) (p:list english_letters{length p < length t}) (i:nat{i <= length t - length p})
-  : bool 
-  = match p with
-    | [] -> true
-    | hd :: tl -> if hd = index t i 
-                  then belongs t tl (i + 1)
-                  else false
+// let rec belongs (t:list english_letters) (p:list english_letters{length p <= length t}) (i:nat)
+//   : bool 
+//   = match p with
+//     | [] -> true
+//     | hd :: tl -> if i < length t && hd = index t i 
+//                   then belongs t tl (i + 1)
+//                   else false
 
 let convert_to_int f =
   match f with
@@ -418,31 +1179,32 @@ let convert_character_to_int (c:english_letters)
   = match c with 
     | A -> 1 
     | B -> 2 
-    | C -> 3
-    | D -> 4
-    | E -> 5
-    | F -> 6
-    | G -> 7
-    | H -> 8
-    | I -> 9
-    | J -> 10
-    | K -> 11
-    | L -> 12
-    | M -> 13
-    | M -> 14
-    | O -> 15
-    | P -> 16
-    | Q -> 17
-    | R -> 18
-    | S -> 19
-    | T -> 20
-    | U -> 21
-    | V -> 22
-    | W -> 23
-    | X -> 24
-    | Y -> 25
-    | Z -> 26
     | _ -> -1
+    // | C -> 3
+    // | D -> 4
+    // | E -> 5
+    // | F -> 6
+    // | G -> 7
+    // | H -> 8
+    // | I -> 9
+    // | J -> 10
+    // | K -> 11
+    // | L -> 12
+    // | M -> 13
+    // | M -> 14
+    // | O -> 15
+    // | P -> 16
+    // | Q -> 17
+    // | R -> 18
+    // | S -> 19
+    // | T -> 20
+    // | U -> 21
+    // | V -> 22
+    // | W -> 23
+    // | X -> 24
+    // | Y -> 25
+    // | Z -> 26
+    // | _ -> -1
 
 let rec convert_letters_to_int (l:list english_letters) : list int =
   match l with
@@ -454,7 +1216,7 @@ let rec convert_letters_to_int (l:list english_letters) : list int =
 
 let main() =
   let message =
-     sprintf "The result is %d\n" (convert_to_int (belongs text pattern 2))
+     sprintf "The result is %s\n" (string_of_int_list (append [1;2;3;4;9] [5;1;2]))
   in
   print_string message
 
